src/impl/TLS13.Impl.ConnectionState.Repr.fst
@@ -426,7 +426,8 @@ fn alloc_server_config_storage
   requires ArrPts.pts_to certificate_chain 'certificate_chain_bytes **
            ArrPts.pts_to credential_identity 'credential_identity_bytes **
            pure (B.length 'certificate_chain_bytes == SZ.v certificate_chain_len /\
-                 B.length 'credential_identity_bytes == SZ.v credential_identity_len)
+                 B.length 'credential_identity_bytes == SZ.v credential_identity_len /\
+                 B.length 'certificate_chain_bytes <= max_server_certificate_chain_len)
   returns cfg:connection_config_storage
   ensures ArrPts.pts_to certificate_chain 'certificate_chain_bytes **
           ArrPts.pts_to credential_identity 'credential_identity_bytes **
@@ -1239,7 +1240,8 @@ fn new_server
   requires ArrPts.pts_to certificate_chain 'certificate_chain_bytes **
            ArrPts.pts_to credential_identity 'credential_identity_bytes **
            pure (B.length 'certificate_chain_bytes == SZ.v certificate_chain_len /\
-                 B.length 'credential_identity_bytes == SZ.v credential_identity_len)
+                 B.length 'credential_identity_bytes == SZ.v credential_identity_len /\
+                 B.length 'certificate_chain_bytes <= max_server_certificate_chain_len)
   returns c:connection_state
   ensures ArrPts.pts_to certificate_chain 'certificate_chain_bytes **
           ArrPts.pts_to credential_identity 'credential_identity_bytes **
